Subst identity when called with `(TmVar x)`

theories/Subst.v
@@ -22,10 +22,47 @@ Proof.
   { reflexivity. } destruct a. rewrite IHa. reflexivity.
 Qed.
 
+Theorem smap_len : forall f li,
+  Datatypes.length (smap f li) = Datatypes.length li.
+Proof.
+  intros f li. generalize dependent f. induction li; intros; simpl in *.
+  { reflexivity. } destruct a. simpl. rewrite IHli. reflexivity.
+Qed.
+
 Theorem map_fst_smap : forall f li,
   map fst (smap f li) = map fst li.
 Proof. induction li. { reflexivity. } destruct a. simpl. rewrite IHli. reflexivity. Qed.
 
+(* Ludicrous that this is the easiest correct definition to write.
+ * Generates substitution functions for every free variable at once. *)
+Fixpoint grand_unified_subst t : list (string * (term -> term)) :=
+  match t with
+  | TmVoid
+  | TmStar
+  | TmAtom _ =>
+      []
+  | TmVarS s =>
+      [(s, fun x => x)]
+  | TmPack id arg ty curry =>
+      smap (fun f x => TmPack id arg (f x) curry) (grand_unified_subst ty) ++
+      smap (fun f x => TmPack id arg ty (f x))
+      match arg, grand_unified_subst curry with
+      | Some a, (s, hd) :: tl => if eqb a s then tl else (s, hd) :: tl
+      | _, passthru => passthru
+      end
+  | TmForA arg ty body =>
+      smap (fun f x => TmForA arg (f x) body) (grand_unified_subst ty) ++
+      smap (fun f x => TmForA arg ty (f x))
+      match arg, grand_unified_subst body with
+      | Some a, (s, hd) :: tl => if eqb a s then tl else (s, hd) :: tl
+      | _, passthru => passthru
+      end
+  | TmAppl a b =>
+      smap (fun f x => TmAppl (f x) b) (grand_unified_subst a) ++
+      smap (fun f x => TmAppl a (f x)) (grand_unified_subst b)
+  end.
+
+(*
 (* Ludicrous that this is the easiest correct definition to write.
  * Generates substitution functions for every free variable at once. *)
 Fixpoint grand_unified_subst t : list (string * (term -> term)) :=
@@ -60,6 +97,7 @@ Fixpoint grand_unified_subst t : list (string * (term -> term)) :=
       | (s, hd) :: tl => if eqb arg s then tl else (s, hd) :: tl
       end
   end.
+*)
 
 Fixpoint pair_lookup {V} key (pairs : list (string * V)) :=
   match pairs with
@@ -80,6 +118,12 @@ Example grand_unified_subst_simple :
     ("x"%string, fun t => TmAppl (TmVarS "f"%string) t)].
 Proof. reflexivity. Qed.
 
+Example grand_unified_subst_lambda :
+  grand_unified_subst (TmForA (Some "x") TmVoid (TmAppl (TmVarS "x") (TmVarS "x")))%string = [
+    (* ignore the first `x`, since it's bound, then *)
+    ("x", fun x => TmForA (Some "x") TmVoid (TmAppl (TmVarS "x") x))%string].
+Proof. reflexivity. Qed.
+
 Theorem grand_unified_subst_exactly_fv : forall t,
   fv t = map fst (grand_unified_subst t).
 Proof.
@@ -91,4 +135,73 @@ Proof.
 Qed.
 (* WOOHOOOOOOOOOOOOOOO *)
 
-(* TODO: Inductive equivalent *)
+Lemma pair_lookup_smap : forall f x li,
+  pair_lookup x (smap f li) = option_map f (pair_lookup x li).
+Proof.
+  intros f x li. generalize dependent x. generalize dependent f.
+  induction li; intros; simpl in *. { reflexivity. }
+  destruct a. simpl. destruct (eqb x s) eqn:E. { reflexivity. } apply IHli.
+Qed.
+
+Lemma pair_lookup_app : forall {T} x a b,
+  @pair_lookup T x (a ++ b) =
+  match pair_lookup x a with
+  | None => pair_lookup x b
+  | Some out => Some out
+  end.
+Proof.
+  intros T x a. generalize dependent x. induction a; intros; simpl in *. { reflexivity. }
+  destruct a. destruct (eqb x s). { reflexivity. } apply IHa.
+Qed.
+
+Lemma pair_lookup_Forall_snd : forall {T} P li x y,
+  Forall P (map snd li) ->
+  @pair_lookup T x li = Some y ->
+  P y.
+Proof.
+  intros T P li x y Hf Hl. generalize dependent y. generalize dependent x.
+  remember (map snd li) eqn:Emap. generalize dependent li.
+  induction Hf; intros; destruct li; invert Emap; try discriminate Hl.
+  destruct p. simpl in *. destruct (eqb x0 s) eqn:E. { invert Hl. assumption. }
+  eapply IHHf; [reflexivity |]. apply Hl.
+Qed.
+
+Lemma pair_lookup_Forall : forall {T} P li x t,
+  Forall P li ->
+  @pair_lookup T x li = Some t ->
+  P (x, t).
+Proof.
+  intros T P li x t Hf Hl. generalize dependent t. generalize dependent x.
+  induction Hf; intros; simpl in *. { discriminate Hl. } destruct x as [k v].
+  destruct (eqb x0 k) eqn:E; [apply eqb_eq in E; invert Hl | apply IHHf]; assumption.
+Qed.
+
+Theorem Forall_smap : forall f P li,
+  Forall (fun p : _ * _ => let (x, g) := p in P (x, f g)) li ->
+  Forall P (smap f li).
+Proof.
+  intros. remember (fun p : string * (term -> term) => let (x, g) := p in P (x, f g)) as F eqn:EF.
+  generalize dependent P. generalize dependent f. induction H; intros; [apply Forall_nil |].
+  destruct x as [s g]. subst. simpl in *. constructor; [assumption |]. apply IHForall. reflexivity.
+Qed.
+
+Theorem grand_unified_subst_id : forall t,
+  let P := fun p : _ * _ => let (x, f) := p in f (TmVarS x) = t in
+  Forall P (grand_unified_subst t).
+Proof.
+  induction t as [| | | | id arg a IHa b IHb | arg a IHa b IHb | a IHa b IHb];
+  subst; simpl in *; try solve [repeat constructor];
+  apply Forall_app; split; apply Forall_smap; try (destruct arg; [
+    destruct (grand_unified_subst b); [constructor |]; destruct p as [x f]; invert IHb;
+    destruct (eqb s x) eqn:E; [| constructor; [reflexivity |]] |]);
+  (eapply Forall_impl; [| try apply IHa; try apply IHb; apply H2]);
+  intros; destruct a0; rewrite H; reflexivity.
+Qed.
+
+Theorem subst_id : forall x t s,
+  subst x (TmVarS x) t = Some s ->
+  s = t.
+Proof.
+  intros. unfold subst in *. destruct (pair_lookup x (grand_unified_subst t)) eqn:Ep; invert H.
+  eapply pair_lookup_Forall in Ep; [| apply grand_unified_subst_id]. assumption.
+Qed.
