theories/Types.v
@@ -70,9 +70,11 @@ Inductive Typed : context -> term -> term -> Prop :=
       ctx = ctxf ++ ctxx ->
       subst arg x body = Some sub ->
       Typed ctx (TmAppl f x) sub
+  (*
   | TyStar : forall ctx t ty,
       Typed ctx t ty ->
       Typed ctx t TmStar
+  *)
   .
 
 (* TODO: CRUCIAL SAFETY THEOREMS: (1) Star does not have type Star, and (2) no term has type Void *)
@@ -108,11 +110,12 @@ Proof.
     ("f"%string, TmForA None (TmVarS "X") (TmForA None (TmVarS "X") (TmVarS "Y")));
     ("x"%string, TmVarS "X")] as ctx eqn:Ec. generalize dependent Ec.
   remember (TmAppl (TmAppl (TmVarS "f") (TmVarS "x")) (TmVarS "x")) as ty eqn:Et. generalize dependent Et.
-  induction C; intros; simpl in *; subst; try discriminate.
-  - invert Et. invert C1; invert H1; invert Ec. destruct ctxx0; invert H3. destruct ctxx; invert H4. invert C2.
-  - invert Et. invert C1; invert H2; invert Ec.
-  - invert C; [| invert H1; invert H3; invert H4 | apply (IHC eq_refl eq_refl)].
-    invert H1; invert H2; invert H5; destruct ctxx0; destruct ctxx; invert H3; invert H6; invert H4.
+  induction C; intros; simpl in *; subst; try discriminate;
+  try (invert Et; invert C1; invert H1; invert Ec; destruct ctxx0; invert H3; destruct ctxx; invert H4; invert C2);
+  try (invert Et; invert C1; invert H2; invert Ec);
+  try (
+    invert C; [| invert H1; invert H3; invert H4 | apply (IHC eq_refl eq_refl)];
+    invert H1; invert H2; invert H5; destruct ctxx0; destruct ctxx; invert H3; invert H6; invert H4).
 Qed.
 
 (* ...But the above becomes perfectly okay if we add exchange and contraction, i.e., a heap: *)
@@ -147,7 +150,7 @@ Qed.
    This might be a crucial lemma in proving type safety (since a void output implies void input)! *)
 
 (* Fantastic that we can prove something this precise! *)
-Theorem typed_requires_fv : forall ctx t ty,
+Theorem typed_free_in : forall ctx t ty,
   Typed ctx t ty -> FreeIn t (map fst ctx).
 Proof.
   intros. induction H; intros; simpl in *; subst; repeat rewrite map_distr; try assumption;
@@ -157,6 +160,222 @@ Qed.
 Theorem fv_not_typed : forall t,
   fv t <> [] -> ~exists ty, Typed [] t ty.
 Proof.
-  intros t H [ty C]. apply typed_requires_fv in C. apply reflect_fv in C.
+  intros t H [ty C]. apply typed_free_in in C. apply reflect_fv in C.
   rewrite C in H. contradiction H. reflexivity.
 Qed.
+
+Theorem typed_fv : forall ctx t ty,
+  Typed ctx t ty ->
+  fv t = map fst ctx.
+Proof. intros. apply reflect_fv. eapply typed_free_in. apply H. Qed.
+
+(* Look up a value by key and remove it from a key-value list. *)
+Fixpoint yoink {T} s (li : list (string * T)) :=
+  match li with
+  | [] => None
+  | (k, v) :: tl => if eqb s k then Some (v, tl) else
+      let f : (T * (list (string * T))) -> _ := fun x =>
+        let (out, etc) := x in (out, (k, v) :: etc) in
+      option_map f (yoink s tl)
+  end.
+
+Example yoink_12345 :
+  yoink "c" [("a", 1); ("b", 2); ("c", 3); ("d", 4); ("e", 5)]%string =
+  Some (3, [("a", 1); ("b", 2); ("d", 4); ("e", 5)]%string).
+Proof. reflexivity. Qed.
+
+Theorem yoink_app : forall {T} s a b out etc,
+  @yoink T s (a ++ b) = Some (out, etc) ->
+  ((exists pre, etc = pre ++ b /\ yoink s a = Some (out, pre)) \/
+  (exists post, etc = a ++ post /\ yoink s a = None /\ yoink s b = Some (out, post))).
+Proof.
+  intros T s a. generalize dependent s. induction a; intros; simpl in *; subst.
+  - right. eexists. repeat split; assumption.
+  - destruct a. destruct (eqb s s0) eqn:E.
+    + apply eqb_eq in E. invert H. left. eexists. repeat split.
+    + destruct (yoink s (a0 ++ b)) eqn:Ey; try discriminate H. destruct p. invert H.
+      apply IHa in Ey. destruct Ey as [[pre [H1 H2]] | [post [H1 [H2 H3]]]]; subst; simpl in *.
+      * left. rewrite H2. eexists; repeat split; try reflexivity.
+      * right. rewrite H2. rewrite H3. eexists; repeat split.
+Qed.
+
+Fixpoint yank {T} i (li : list T) :=
+  match li with
+  | [] => None
+  | hd :: tl =>
+      match i with
+      | O => Some (hd, tl)
+      | S j => 
+          let f := fun x : _ * _ => let (out, etc) := x in (out, hd :: etc) in
+          option_map f (yank j tl)
+      end
+  end.
+
+Fixpoint checked_sub amt from :=
+  match from, amt with
+  | _, O => Some from
+  | S f, S a => checked_sub a f
+  | _, _ => None
+  end.
+
+Example checked_sub_3_5 : checked_sub 3 5 = Some 2. Proof. reflexivity. Qed.
+Example checked_sub_5_3 : checked_sub 5 3 = None. Proof. reflexivity. Qed.
+
+Theorem checked_sub_le : forall amt from,
+  checked_sub amt from <> None <-> amt <= from.
+Proof.
+  induction amt; intros; simpl in *.
+  - split; intros. { apply le_0_n. } intro C. destruct from; discriminate C.
+  - split; intros; destruct from; try contradiction. { apply le_n_S. apply IHamt. assumption. }
+    { invert H. } apply le_S_n in H. apply IHamt. assumption.
+Qed.
+
+Theorem checked_sub_sub : forall amt from out,
+  checked_sub amt from = out ->
+  from - amt = match out with Some x => x | None => O end.
+Proof.
+  induction amt; intros; simpl in *. { destruct from; invert H; reflexivity. }
+  destruct from; subst; simpl in *. { reflexivity. } apply IHamt. reflexivity.
+Qed.
+
+Theorem yank_app : forall {T} i a b,
+  @yank T i (a ++ b) =
+  match checked_sub (Datatypes.length a) i with
+  | None =>
+      let f : _ * _ -> _ := fun x => let (out, etc) := x in (out, etc ++ b) in
+      option_map f (yank i a)
+  | Some past_a =>
+      let f : _ * _ -> _ := fun x => let (out, etc) := x in (out, a ++ etc) in
+      option_map f (yank past_a b)
+  end.
+Proof.
+  intros T i a. generalize dependent i. induction a; intros; simpl in *.
+  - destruct i; destruct b; simpl; try reflexivity.
+    destruct (yank i b); simpl; try reflexivity. destruct p. reflexivity.
+  - destruct i; simpl in *. { reflexivity. } rewrite IHa. clear IHa.
+    destruct (checked_sub (Datatypes.length a0) i); simpl in *.
+    + destruct (yank n b); simpl; try reflexivity. destruct p. reflexivity.
+    + destruct (yank i a0); try reflexivity. destruct p. reflexivity.
+Qed.
+
+Lemma nth_error_short_circuit : forall {T} i a b out,
+  @nth_error T a i = Some out ->
+  nth_error (a ++ b) i = Some out.
+Proof.
+  intros T i a. generalize dependent i. induction a; intros; simpl in *. { destruct i; discriminate H. }
+  destruct i; simpl in *. { invert H. reflexivity. } apply IHa. assumption.
+Qed.
+
+Lemma nth_error_smap : forall f li i,
+  nth_error (smap f li) i = option_map (fun pair : _ * _ => let (a, b) := pair in (a, f b)) (nth_error li i).
+Proof.
+  intros f li. generalize dependent f. induction li; intros; simpl in *. { destruct i; reflexivity. }
+  destruct a. destruct i; simpl in *. { reflexivity. } apply IHli.
+Qed.
+
+(*
+Theorem grand_unified_subst_preserves_typing : forall ctx t ty,
+  Typed ctx t ty ->
+  forall i s st ctx',
+  yank i ctx = Some ((s, st), ctx') ->
+  exists f,
+  nth_error (grand_unified_subst t) i = Some (s, f) /\
+  forall y,
+  Typed [] y st ->
+  Typed ctx' (f y) ty.
+Proof.
+  intros ctx t ty H. induction H; intros; simpl in *; subst.
+  - destruct i; [| destruct i; discriminate]. invert H. eexists. repeat split. intros. assumption.
+  - destruct i; discriminate H.
+  - rewrite yank_app in H3. destruct (checked_sub (Datatypes.length ctxt) i) eqn:Ec;
+    [destruct (yank n ctxc) eqn:Ey | destruct (yank i ctxt) eqn:Ey]; try discriminate H3; destruct p; invert H3.
+    + admit.
+    + destruct arg.
+      * admit.
+      * eapply IHTyped1 in Ey as [f [E1 E2]]. clear IHTyped1; clear IHTyped2.
+        erewrite nth_error_short_circuit; [| rewrite nth_error_smap; rewrite E1; reflexivity].
+        eexists; repeat split. intros. apply E2 in H1. simpl. eapply TyPack. Print Typed. econstructor. assumption.
+        rewrite nth_error_smap. rewrite E1; reflexivity.
+
+    + assert (A : checked_sub (Datatypes.length ctxt) i <> None). { rewrite Ec. intro C. discriminate C. }
+      apply checked_sub_le in A. destruct arg.
+      * rewrite nth_error_app2; rewrite smap_len; assert (F := typed_fv _ _ _ H);
+        rewrite grand_unified_subst_exactly_fv in F; eassert (L := f_equal _ F);
+        repeat rewrite map_length in L; rewrite L; try assumption.
+        clear IHTyped1; clear IHTyped2. eexists. split.
+        -- rewrite (checked_sub_sub _ _ _ Ec).
+  - destruct arg.
+    + clear IHTyped1; clear IHTyped2.
+
+    + admit.
+    + rewrite yank_app in H3. destruct (checked_sub (Datatypes.length ctxt) i) eqn:Ec.
+      * destruct (yank n ctxc) eqn:Ey; try discriminate H3. destruct p. destruct p. invert H3.
+        apply IHTyped2 in Ey as [f [E1 E2]].
+        assert (A : checked_sub (Datatypes.length ctxt) i <> None). { rewrite Ec. intro C. discriminate C. }
+        apply checked_sub_le in A. eexists. rewrite nth_error_app2; [|
+          rewrite smap_len; apply typed_fv in H; rewrite grand_unified_subst_exactly_fv in H;
+          eapply f_equal in H; repeat rewrite map_length in H; rewrite H; assumption].
+        split. admit. intros. simpl in *. clear IHTyped1; clear IHTyped2.
+
+    + rewrite yank_app in H3. destruct (checked_sub (Datatypes.length ctxt) i). clear IHTyped1; clear IHTyped2.
+  - rewrite yank_app in H3. destruct (checked_sub (Datatypes.length ctxt) i) eqn:E.
+    + destruct (yank n ctxc) eqn:Ey; try discriminate H3. clear IHTyped1; clear IHTyped2. destruct p. invert H3. destruct arg.
+      * admit.
+      * assert (A := checked_sub_le (Datatypes.length ctxt) i).
+      * apply checked_sub_le in E. Search nth_error. simpl in *.
+
+  - clear IHTyped1; clear IHTyped2. assert (A := typed_fv _ _ _ H). rewrite grand_unified_subst_exactly_fv in A. destruct arg.
+    + admit.
+    + 
+
+  intros ctx. induction ctx; intros; simpl in *. { destruct i; discriminate H0. }
+  Search fv.
+  assert (A := typed_fv _ _ _ H).
+  rewrite grand_unified_subst_exactly_fv in A.
+  destruct a.
+  apply grand_unified_subst_exactly_fv 
+  Search grand_unified_subst.
+  apply IHctx.
+Qed.
+
+Theorem grand_unified_subst_preserves_typing : forall ctx t ty,
+  (* A mouthful: if you substitute a variable in context with something of its assigned type,
+   * and if you then remove that variable from the context,
+   * then the type of the whole expression after substitution doesn't change. *)
+  Typed ctx t ty ->
+  forall x xt ctx',
+  yoink x ctx = Some (xt, ctx') ->
+  forall y,
+  Typed [] y xt ->
+  exists s,
+  subst x y t = Some s /\ Typed ctx' s ty.
+Proof.
+  intros ctx t ty H. induction H; intros; simpl in *; subst; try discriminate.
+  - destruct (eqb x id) eqn:E; invert H. apply eqb_eq in E. subst. simpl in *.
+    eexists. split. { reflexivity. } assumption.
+  - apply yoink_app in H3. destruct H3 as [[pre [E1 E2]] | [post [E1 [E2 E3]]]].
+    + eapply IHTyped1 in E2 as [s [E2 E3]]. clear IHTyped1; clear IHTyped2. subst. destruct arg.
+    + clear IHTyped1; clear IHTyped2. simpl in *.
+Qed.
+
+Theorem subst_preserves_typing : forall x y t ty s,
+  Typed [] t ty ->
+  subst x y t = Some s ->
+  Typed [] s ty.
+Proof.
+  intros x y t. generalize dependent y. generalize dependent x.
+  induction t; intros; simpl in *; try discriminate.
+  - apply typed_fv in H. discriminate H.
+  - invert H. destruct ctxt; destruct ctxc; invert H9. clear H0. destruct arg.
+    + admit.
+    + eapply IHt2.
+
+  - assert (A := fv_not_typed (TmVarS id)). contradiction A. { intro C. discriminate C. } exists ty. assumption.
+  - clear H0. induction H.
+    + eapply IHt2.
+  - destruct arg.
+    + clear H0. invert H. simpl in *.
+
+  - destruct (eqb x id) eqn:E; invert H0. apply eqb_eq in E. subst. induction H.
+Qed.
+*)
