theories/TypeSafety.v
@@ -1,0 +1,44 @@
+From Lang Require Import
+  Invert
+  Terms
+  Types.
+
+Theorem no_type_in_type : forall ctx,
+  ~Typed ctx TmStar TmStar.
+Proof.
+  intros ctx C. remember TmStar as t eqn:Et. remember TmStar as ty eqn:Ety. rewrite Et in C at 2.
+  induction C; intros; simpl in *; subst; try discriminate.
+  (* inversion C. subst. apply IHC; reflexivity. *)
+Qed.
+
+(*
+Theorem BAD_exists_term_typed_void : exists t,
+  Typed [] t TmVoid.
+Proof.
+  eexists. Check TyApplNone. eapply (TyApplNone [] [] [] _ _ (TmAtom "")); try reflexivity.
+  - econstructor. { constructor. }
+  - eapply (TyApplNone [] [] []); try reflexivity.
+Qed.
+
+Theorem no_term_typed_void : forall t,
+  ~Typed [] t TmVoid.
+Proof.
+  intros t C. remember TmVoid as ty eqn:Et. remember [] as ctx eqn:Ec.
+  generalize dependent Ec. generalize dependent Et. induction C; intros; simpl in *; subst; try discriminate;
+  (* At this point, only function application is left *)
+  destruct ctxf; destruct ctxx; invert Ec.
+  - clear IHC1. induction ty; try apply (IHC2 eq_refl eq_refl); clear IHC2.
+    + 
+  - clear IHC1. invert C1; try (destruct ctxt; destruct ctxc; invert H6).
+    + clear IHC1.
+
+  - clear IHC1. generalize dependent x. generalize dependent IHC2.
+    remember [] as ctx eqn:Ec. generalize dependent Ec.
+    remember (TmForA None ty TmVoid) as fora eqn:Ef. generalize dependent ty.
+    induction C1; intros; simpl in *; try discriminate.
+    + invert Ef. clear IHC1_2. destruct ctxt; destruct ctxc; invert Ec; simpl in *.
+      apply IHC2; try reflexivity.
+      eapply IHC1_1; try reflexivity.
+    + destruct ctxt; destruct ctxc; invert H6.
+Qed.
+*)
