flake.nix
@@ -1,7 +1,6 @@
 {
   description = "Fast, pure, dependently typed language.";
   inputs = {
-    # array.url = "github:wrsturgeon/array";
     flake-utils.url = "github:numtide/flake-utils";
     nixpkgs.url = "github:nixos/nixpkgs/nixos-unstable";
   };
@@ -14,12 +13,10 @@
         src = ./.;
         os-pkgs = import nixpkgs { inherit system; };
         pkgs = os-pkgs.coqPackages;
-        # flakes = map (p: p.packages.${system}.default);
       in {
         packages.default = pkgs.mkCoqDerivation {
           inherit pname version owner src;
           buildInputs = with os-pkgs; [ ocaml ];
-          # propagatedBuildInputs = flakes [ array ];
         };
       });
 }
